Added receive functions to connection table experiment

src/tls/experiments/ConnectionTable3.fst
@@ -12,19 +12,25 @@ module DM = FStar.DependentMap
 
 type connection_id = nat
 
+assume val configuration: Type0
+
 assume val client_hello: Type0
+
+assume val ch_random: ch:client_hello -> nat
 
 assume val cookie : Type0
 
 assume val has_cookie: client_hello -> bool
 
-assume val ch_cookie: ch:client_hello{has_cookie ch} -> cookie
+assume val ch_of_cookie: ch:client_hello{has_cookie ch} -> client_hello
 
-assume val matches: cookie -> client_hello -> Type0
+assume val ch_compatible: client_hello -> configuration -> bool
+
+assume val rgn:erid
 
 noeq
 type connection =
-  | Init: connection
+  | Init: cfg:configuration -> connection
   | Sent_HRR: random:nat -> ch:client_hello -> connection
   | Sent_ServerHello: random:nat -> ch:client_hello -> id1:connection_id -> connection
   | Complete: random:nat -> ch:client_hello -> id1:connection_id -> connection
@@ -33,27 +39,14 @@ let nonce_of (c:connection{~(Init? c)}) =
   match c with
   | Sent_HRR r _ | Sent_ServerHello r _ _ | Complete r _ _ -> r
 
-let ch_of (c:connection{~(Init? c)}) =
-  match c with
-  | Sent_HRR _ ch | Sent_ServerHello _ ch _ | Complete _ ch _ -> ch
-
-let cookie_of (c:connection{~(Init? c) /\ has_cookie (ch_of c)}) =
-  ch_cookie (ch_of c)
-
-let id0_of (c:connection{Sent_ServerHello? c \/ Complete? c}) =
-  match c with
-  | Sent_ServerHello _ _ id0 | Complete _ _ id0 -> id0
-
 let step (s1 s2:connection) : Type0 =
   match s1, s2 with
-  | Init, Sent_HRR _ _ -> True
-  | Init, Sent_ServerHello _ _ _ -> True
+  | Init _, Sent_HRR _ _ -> True
+  | Init _, Sent_ServerHello _ _ _ -> True
   | Sent_ServerHello r ch id0, Complete r' ch' id0' -> r == r' /\ ch == ch' /\ id0 == id0'
   | _, _ -> False
 
 let rel : Preorder.preorder connection = closure step
-
-assume val rgn:erid
 
 let connection_ref (id:connection_id) = r:mmmref connection rel{frameOf r `extends` rgn}
 
@@ -77,7 +70,7 @@ let connection_inv m c =
         token_p c' (fun h0 -> 
           Sent_HRR? (sel h0 c') /\ 
           nonce_of (sel h0 c') == r /\
-          ch_cookie ch `matches` Sent_HRR?.ch (sel h0 c'))
+          ch_of_cookie ch == Sent_HRR?.ch (sel h0 c'))
       | _ -> False
     else True
   | _ -> True
@@ -90,7 +83,7 @@ val inv: t:connection_table -> h:mem -> Type0
 let inv t h = 
   let m = sel h t in
   forall (id:connection_id).{:pattern (T.defined t id h)}
-    (T.defined t id h /\ h `contains` (T.value_of t id h))    
+    (T.defined t id h /\ h `contains` (T.value_of t id h))
     ==> connection_inv m (sel h (Some?.v (T.sel m id)))
 
 val alloc: unit -> ST (connection_table)
@@ -99,23 +92,24 @@ val alloc: unit -> ST (connection_table)
 let alloc _ =
   T.alloc ()
 
-val create: t:connection_table -> id:connection_id -> ST (connection_ref id)
-  (requires fun h0 -> h0 `contains` t /\ inv t h0 /\ ~(T.defined t id h0))
+val create: t:connection_table -> id:connection_id -> cfg:configuration 
+  -> ST (connection_ref id)
+  (requires fun h0 -> inv t h0 /\ ~(T.defined t id h0))
   (ensures  fun h0 c h1 -> 
     mods [Ref t] h0 h1 /\ 
-    h1 `contains` t /\ 
     inv t h1 /\
     T.defined t id h1 /\
     sel h1 t == T.upd (sel h0 t) id c /\
     ~(h0 `contains` c) /\
     h1 `contains` c /\
-    sel h1 c == Init)
-let create t id =
+    sel h1 c == Init cfg)
+let create t id cfg =
+  recall t; 
   let h0 = get () in
   let p (id:connection_id{T.defined t id h0}) = frameOf (T.value_of t id h0) in
   testify_forall_region_contains_pred #_ #p ();
   let rgn1 = new_region rgn in
-  let c : mmmref connection rel = ralloc_mm rgn1 Init in
+  let c : mmmref connection rel = ralloc_mm rgn1 (Init cfg) in
   let h1 = get () in
   assert (forall (id:connection_id). T.defined t id h0 ==> ~(c == T.value_of t id h0));
   assert (inv t h1);
@@ -129,7 +123,7 @@ let create t id =
 
 val free: t:connection_table -> id:connection_id -> ST unit
   (requires fun h0 -> 
-    h0 `contains` t /\ inv t h0 /\ T.defined t id h0 /\
+    inv t h0 /\ T.defined t id h0 /\
     T.value_of t id h0 `is_live_for_rw_in` h0 /\ inv t h0)
   (ensures  fun h0 _ h1 -> 
     h0 `contains` (T.value_of t id h0) /\
@@ -154,6 +148,126 @@ val token_functoriality
    [SMTPat (token_p r p); SMTPat (token_p r q)]
 let token_functoriality #a #rel r p q = 
   token_functoriality r p q
+  
+val receive_client_hello1: 
+    t:connection_table 
+  -> id:connection_id 
+  -> ch:client_hello{~(has_cookie ch)}
+  -> ST unit
+  (requires fun h0 -> 
+    T.defined t id h0 /\ 
+    h0 `contains` T.value_of t id h0 /\ 
+    inv t h0 /\
+    Init? (sel h0 (T.value_of t id h0)))
+  (ensures  fun h0 _ h1 -> 
+    inv t h1 /\ 
+    T.defined t id h1 /\
+    mods [Ref (T.value_of t id h0)] h0 h1 /\
+    (if ch_compatible ch (Init?.cfg (sel h0 (T.value_of t id h0))) then
+      sel h1 (T.value_of t id h1) == Sent_ServerHello (ch_random ch) ch 0
+    else 
+      sel h1 (T.value_of t id h1) == Sent_HRR (ch_random ch) ch))
+let receive_client_hello1 t id ch =
+  let h0 = get () in
+  let c = Some?.v (T.lookup t id) in  
+  if ch_compatible ch (Init?.cfg !c) then
+    c := Sent_ServerHello (ch_random ch) ch 0
+  else 
+    c := Sent_HRR (ch_random ch) ch;
+  let h1 = get () in
+  assert (
+    let m = sel h1 t in
+    forall (id:connection_id).{:pattern (T.defined t id h1)}
+    (T.defined t id h0 /\ h1 `contains` (T.value_of t id h1)) ==> 
+    connection_inv m (sel h1 (T.value_of t id h1)))
+
+(* 
+   Validates a cookie and returns the id of the connection where it originates, if valid.
+   Ideally, we can enforce that authentic cookies come from an earlier honest connection.
+*)
+assume
+val id_of_cookie:
+  t:connection_table ->
+  ch:client_hello{has_cookie ch} ->
+  ST (option connection_id)
+  (requires fun h0 -> inv t h0)
+  (ensures  fun h0 o h1 ->
+    match o with
+    | None -> h0 == h1
+    | Some id0 ->
+      h0 == h1 /\
+      T.defined t id0 h0 /\
+      (let c' = T.value_of t id0 h0 in
+       token_p c' (fun h0 -> 
+         Sent_HRR? (sel h0 c') /\ 
+         nonce_of (sel h0 c') == ch_random ch /\
+         ch_of_cookie ch == Sent_HRR?.ch (sel h0 c'))))
+
+val receive_client_hello2: 
+    t:connection_table 
+  -> id:connection_id 
+  -> ch:client_hello 
+  -> ST bool
+  (requires fun h0 -> 
+    T.defined t id h0 /\ h0 `contains` T.value_of t id h0 /\ inv t h0 /\
+    Init? (sel h0 (Some?.v (T.sel (sel h0 t) id))) /\ has_cookie ch)
+  (ensures  fun h0 b h1 -> 
+    inv t h1 /\
+    T.defined t id h1 /\
+    mods [Ref (T.value_of t id h0)] h0 h1 /\
+    (let c' = sel h1 (T.value_of t id h1) in
+    b ==>    
+      Sent_ServerHello? c' /\
+      Sent_ServerHello?.random c' == ch_random ch /\
+      Sent_ServerHello?.ch c' == ch))
+let receive_client_hello2 t id ch =
+  let h0 = get () in
+  let c = Some?.v (T.lookup t id) in 
+  match id_of_cookie t ch with
+  | None -> false
+  | Some id0 ->
+    if ch_compatible ch (Init?.cfg !c) then
+      begin
+      c := Sent_ServerHello (ch_random ch) ch id0;
+      let h1 = get () in
+      assert (
+        let m = sel h1 t in
+        forall (id:connection_id).{:pattern (T.defined t id h1)}
+        (T.defined t id h0 /\ h1 `contains` (T.value_of t id h1)) ==> 
+        connection_inv m (sel h1 (T.value_of t id h1)));
+      true
+      end
+    else false
+
+val receive_client_finished: 
+    t:connection_table 
+  -> id:connection_id 
+  -> ST unit
+  (requires fun h0 -> 
+    T.defined t id h0 /\ h0 `contains` T.value_of t id h0 /\ inv t h0 /\
+    Sent_ServerHello? (sel h0 (Some?.v (T.sel (sel h0 t) id))))
+  (ensures  fun h0 b h1 -> 
+    inv t h1 /\
+    T.defined t id h1 /\
+    mods [Ref (T.value_of t id h0)] h0 h1 /\
+    (let c0 = sel h0 (T.value_of t id h0) in
+     let c1 = sel h1 (T.value_of t id h1) in
+     Complete? c1 /\
+     Complete?.random c1 == Sent_ServerHello?.random c0 /\
+     Complete?.ch c1 == Sent_ServerHello?.ch c0))
+let receive_client_finished t id =
+  let c = Some?.v (T.lookup t id) in
+  let c0 = !c in
+  let h0 = get() in
+  c := Complete (Sent_ServerHello?.random c0) 
+               (Sent_ServerHello?.ch c0) 
+               (Sent_ServerHello?.id1 c0);
+  let h1 = get () in
+  assert (
+    let m = sel h1 t in
+    forall (id:connection_id).{:pattern (T.defined t id h1)}
+      (T.defined t id h0 /\ h1 `contains` (T.value_of t id h1)) ==> 
+      connection_inv m (sel h1 (T.value_of t id h1)))
 
 #set-options "--z3rlimit 100"
 
@@ -166,31 +280,26 @@ let token_functoriality #a #rel r p q =
    4. Deallocate c1
    5. Create a second connection c2 (in Init state)
    6. Receive a ClientHello ch2 on c2 with a random and cookie extension matching ch1.
-      Transition c2 to Sent_ServerHello 0 ch2 1, with c1 as the matching initial connection 
-   7. Receive a ClientFinished on c2. Transition c2 to Complete 0 ch2 1
+   7. If the configuration of c2 is compatible with ch2,
+      a. Transition c2 to Sent_ServerHello 0 ch2 1, with c1 as the matching initial connection
+      b. Receive a ClientFinished on c2. Transition c2 to Complete 0 ch2 1
    8. Deallocate c2
 *)
-val test: ch1:client_hello -> ch2:client_hello{has_cookie ch2} -> ST connection_table
-  (requires fun _ -> witnessed (region_contains_pred rgn) /\
-                  ch_cookie ch2 `matches` ch1)
-  (ensures  fun h0 t h1 -> h1 `contains` t /\ inv t h1)
-let test ch1 ch2 =
+val test: 
+    cfg:configuration
+  -> ch1:client_hello{~(has_cookie ch1) /\ ch_random ch1 == 0} 
+  -> ch2:client_hello{has_cookie ch2 /\ ch_random ch2 == 0} 
+  -> ST connection_table
+  (requires fun _ -> 
+    witnessed (region_contains_pred rgn) /\ ch_of_cookie ch2 == ch1 /\
+    ~(ch_compatible ch1 cfg))
+  (ensures  fun h0 t h1 -> inv t h1)
+let test cfg ch1 ch2 =
   let t = alloc () in
-  let c1 = create t 1 in
-  c1 := Sent_HRR 0 ch1;
-  stable_on_closure (closure step) 
-    (fun c ->
-      Sent_HRR? c /\ 
-      nonce_of c == 0 /\
-      ch_cookie ch2 `matches` Sent_HRR?.ch c) ();
-  witness_p c1 
-    (fun h -> 
-      Sent_HRR? (sel h c1) /\ 
-      nonce_of (sel h c1) == 0 /\
-      ch_cookie ch2 `matches` Sent_HRR?.ch (sel h c1));
+  let c1 = create t 1 cfg in
+  receive_client_hello1 t 1 ch1;  
   free t 1;
-  let c2 = create t 2 in
-  c2 := Sent_ServerHello 0 ch2 1;
-  c2 := Complete 0 ch2 1;  
+  let c2 = create t 2 cfg in
+  if receive_client_hello2 t 2 ch2 then receive_client_finished t 2;
   free t 2;
   t
